Separate out nnrc_imp_eval/sem

coq/NNRCimp/Lang/NNRCimpEval.v
@@ -172,18 +172,25 @@ Section NNRCimpEval.
            end
          end.
 
-    Definition nnrc_imp_eval_top σc (q:nnrc_imp) :=
+    Definition nnrc_imp_eval σc (q:nnrc_imp) : option (option data) :=
       let (s, ret) := q in
       match nnrc_imp_stmt_eval (rec_sort σc) nil nil ((ret, None)::nil) s with
-      | Some (_, _, (_,Some d)::_) => Some d
+      | Some (_, _, (_,o)::_) => Some o
       | _ => None
       end.
+
+    Definition nnrc_imp_eval_top σc (q:nnrc_imp) :=
+      olift id (nnrc_imp_eval σc q).
 
   End Evaluation.
 
   Section Core.
+    Program Definition nnrc_imp_core_eval σc (q:nnrc_imp_core)
+      := nnrc_imp_eval σc q.
+
     Program Definition nnrc_imp_core_eval_top σc (q:nnrc_imp_core)
-      := nnrc_imp_eval_top σc q.
+      :=  olift id (nnrc_imp_core_eval σc q).
+    
   End Core.
 
   Section props.
